

APPENDIX.A

We present detailed estimates of

$$\sum_{\mathbf{y} \in \Sigma_q^{n-tb}} |D_t^b(\mathbf{y})|^{-1},$$

which were omitted in Section IV, and which complete the proof of the upper bound on $M_q(n, (t, b))$.

Note that

$$\sum_{\mathbf{y} \in \Sigma_q^{n-tb}} |D_t^b(\mathbf{y})|^{-1} = \sum_{r=1}^{n-(t+1)b+1} \sum_{\substack{\mathbf{y} \in \Sigma_q^{n-tb} \\ |U_b(\mathbf{y})|=r}} |D_t^b(\mathbf{y})|^{-1}.$$

Thus, by the lower bound on $|D_t^b(\mathbf{y})|$ in Theorem 2, we have

$$\begin{aligned} & \sum_{\mathbf{y} \in \Sigma_q^{n-tb}} |D_t^b(\mathbf{y})|^{-1} \\ & \leq \sum_{r=r'+1}^{n-(t+1)b+1} \sum_{\substack{\mathbf{y} \in \Sigma_q^{n-tb} \\ |U_b(\mathbf{y})|=r}} \binom{r-(t-1)b}{t}^{-1} \\ & \quad + \sum_{r=1}^{r'} \sum_{\substack{\mathbf{y} \in \Sigma_q^{n-tb} \\ |U_b(\mathbf{y})|=r}} 1 \\ & = \sum_{r=r'+1}^{n-(t+1)b+1} \frac{|\{\mathbf{y} \in \Sigma_q^{n-tb} : |U_b(\mathbf{y})|=r\}|}{\binom{r-(t-1)b}{t}} \\ & \quad + \sum_{r=1}^{r'} |\{\mathbf{y} \in \Sigma_q^{n-tb} : |U_b(\mathbf{y})|=r\}| \\ & = q^b \sum_{r=r'+1}^{n-(t+1)b+1} (q-1)^{r-1} \frac{\binom{n-tb-b}{r-1}}{\binom{r-(t-1)b}{t}} \end{aligned} \quad (15)$$

$$+ q^b \sum_{r=1}^{r'} (q-1)^{r-1} \binom{n-tb-b}{r-1}, \quad (16)$$

where $r' \geq (t-1)(b+1)$ is a parameter to be determined later, and the last equality follows from

$$|\{\mathbf{y} \in \Sigma_q^{n-tb} : |U_b(\mathbf{y})|=r\}| = \binom{n-tb-b}{r-1} q^b (q-1)^{r-1},$$

see Claim 4 in Appendix A of [13] for a detailed proof.

To further estimate (15) and (16), we consider the following binomial random variable $X \sim \text{Binomial}(N, \theta)$ with parameters $N = n - (t+1)b$ and $\theta = \frac{q-1}{q}$. The expectation of X is $\mu \triangleq \mathbb{E}(X) = N\theta$ and the variance is $\text{Var}(X) = N\theta(1-\theta)$. Moreover, by the Chernoff bound, it holds that

$$\Pr(X \geq (1-\epsilon)\mu) \leq e^{-\frac{\epsilon^2\mu}{2}}.$$

The term in (16) can be simplified as

$$\begin{aligned} & q^b \sum_{r=0}^{r'-1} (q-1)^r \binom{N}{r} \\ & = q^{N+b} \sum_{r=0}^{r'-1} \binom{N}{r} \left(1 - \frac{1}{q}\right)^r \left(\frac{1}{q}\right)^{N-r} \\ & = q^{N+b} \Pr(X < r'). \end{aligned} \quad (17)$$

Moreover, since $\binom{r-(t-1)b}{t}$ is monotone increasing in r , thus the term in (15) can be simplified as

$$\begin{aligned} & q^b \sum_{r=r'+1}^{n-(t+1)b+1} (q-1)^{r-1} \frac{\binom{n-tb-b}{r-1}}{\binom{r-(t-1)b}{t}} \\ & \leq \frac{q^b}{\binom{r'+1-(t-1)b}{t}} \sum_{r=r'+1}^{n-(t+1)b+1} (q-1)^{r-1} \binom{n-tb-b}{r-1} \\ & = \frac{q^b}{\binom{r'+1-(t-1)b}{t}} \sum_{r=r'}^N (q-1)^r \binom{N}{r} \\ & \leq \frac{q^{N+b}}{\binom{r'+1-(t-1)b}{t}}, \end{aligned} \quad (18)$$

where the last inequality follows by $\sum_{r=r'}^N (q-1)^r \binom{N}{r} \leq q^N$.

Setting $r' = \mu - \sqrt{2tN \ln N}$ in (18) and (17), then by the Chernoff bound, the RHS of (17) is at most

$$\begin{aligned} & q^{N+b} \cdot e^{-\frac{tN \ln N}{\mu}} \leq \frac{q^{N+b}}{N^{\frac{tq}{q-1}}} \\ & = o\left(\frac{q^{n-tb}}{(n-(t+1)b)^t}\right), \end{aligned}$$

as $n \rightarrow \infty$. Meanwhile, by

$$\begin{aligned} & \binom{r'+1-(t-1)b}{t} \geq \frac{(\mu - (t-1)b)^t}{t!} (1 - o(1)) \\ & = \left(\frac{q-1}{q}\right)^t \left(n - 2tb - \frac{(t-1)b}{q}\right)^t \frac{1}{t!} (1 - o(1)) \end{aligned} \quad (19)$$

as $n \rightarrow \infty$, the RHS of (18) is at most

$$\frac{q^{N+b+t} t!}{(q-1)^t \left(n - 2tb - \frac{(t-1)b}{q}\right)^t} (1 + o(1)).$$

In total, this leads to

$$\begin{aligned} & \sum_{\mathbf{y} \in \Sigma_q^{n-tb}} |D_t^b(\mathbf{y})|^{-1} \\ & \leq \frac{t! q^{n-tb+t}}{(q-1)^t \left(n - 2tb - \frac{(t-1)b}{q}\right)^t} (1 + o(1)) \end{aligned}$$

and confirms the upper bound in Theorem 1.